---
title: "AMHG"
author: "Mark Hagemann"
date: "November 16, 2017"
output: html_document
---

```{r setup, include=FALSE}
knitr::opts_chunk$set(echo = TRUE)
```


### AMHG

At-many-stations hydraulic geometry [@Gleason2014] can be expressed as:

$$
\log Q_t = \frac{1}{b_i} (\log W_{it} - \log{W_c}) + \log Q_c
$$
{#eq:AMHG1}

Rewritten to isolate the observed variable, $\log W_{it}$, this is:

$$
\log W_{it} = b_i (\log Q_{t} - \log{Q_c}) + \log W_c
$$

For simplicity, define the following:

- $y_{it} = \log W_{it}$
- $\tilde{b}_i = b_i - \bar{b}$
- $\tilde{q_t} = \log Q_t - E[{\log Q}]$
- $\tilde{q_c} = \log Q_c - E[{\log Q}]$
- $\tilde{w}_c = \log W_c$
- $\gamma_{it} = b_i$

Then, 

$$
\begin{aligned}
\tilde{y}_{it} &= b_i (\log Q_{t} - \log{Q_c}) + \log W_c \\ 
& = b_i (\tilde{q_t} - \tilde{q_c}) + \tilde{w}_c \\ 
& = (\tilde{b}_i + \bar{b})(\tilde{q_t} - \tilde{q_c}) + \tilde{w}_c \\ 
& = \gamma_{it} + \alpha_i + \beta_t + \mu \\ 
\end{aligned}
$$

where

- $\gamma_{it} = (b_i - \bar{b})(\log Q_t - E[\log Q])$
- $\alpha_i = (b_i - \bar{b})(\log Q_c - E[{\log Q}])$
- $\beta_t = $



